added new lemmas

hashedelgamal.ec
@@ -1,5 +1,3 @@
-(* Hashed el'gamal proof *)
-
 require import AllCore Distr SmtMap DBool FSet.
 
 type group.
@@ -61,9 +59,9 @@ lemma gen_log : cancel gen log.
       have choice_g2q := choicebP ( gen_rel(g ^ q)) e.
       have /choice_g2q @/gen_rel/inj {2}-> //:
       exists(q' : exp), gen_rel (g^q) q'
-      by rewrite /gen_rel; by exists q.        
+      by rewrite /gen_rel; by exists q.       
   qed.
-  
+
 lemma log_gen : cancel log gen.
     proof.
       rewrite /gen /log /cancel => x.
@@ -74,7 +72,7 @@ lemma log_gen : cancel log gen.
 lemma grexpAll (x : group) (q1 q2 : exp) : (x ^ q1) ^q2 = x ^ (q1 * q2).
     proof.
       have ->: x = g ^ log x.
-      have ->: g ^ log x = gen (log x).    
+      have ->: g ^ log x = gen (log x).   
       by rewrite /gen.
       by rewrite log_gen.
      by rewrite !grexpA expA.
@@ -147,16 +145,16 @@ module RO : RO = {
 
 module Cor (Enc : ENC) = {
   module E = Enc(RO)
-  
+
   proc main(x : text) : bool = {
   var pubk : group; var privk : exp; var c : cipher; var y : text;
-    
+
     (pubk, privk) <@ E.key_gen();
       c <@ E.enc(pubk, x);
       y <@ E.dec(privk, c);
     return x = y;
   }
-  
+
 }.
 
 
@@ -171,7 +169,7 @@ module (HEG : ENC) (RO : RO) ={
       var r : exp;
     var u : text;
     r <$ dexp;
-    
+
       (* Need to define pubk and privk. pubk = g ^ q and privk = q *)
     u <@ RO.f(pubk ^ r);
 
@@ -206,7 +204,7 @@ lemma correctness : phoare[Cor(HEG).main : true ==> res] = 1%r.
     proof.
       proc.
     inline*.
-    seq 13: (x1 = g ^ (q * r) /\ x2 = x1 /\ t = x /\ RO.mp.[x1] = Some u /\ u0 = t +^ u).  
+    seq 13: (x1 = g ^ (q * r) /\ x2 = x1 /\ t = x /\ RO.mp.[x1] = Some u /\ u0 = t +^ u). 
     auto.
     seq 3: (pubk0 = g ^ q /\ privk = q).
     wp.
@@ -219,7 +217,7 @@ lemma correctness : phoare[Cor(HEG).main : true ==> res] = 1%r.
     seq 2: (pubk0 = g ^ q /\ privk = q /\ t = x).
     auto.
     auto.
-    progress. 
+    progress.
     apply dexp_ll.
     sp.
     if.
@@ -227,7 +225,7 @@ lemma correctness : phoare[Cor(HEG).main : true ==> res] = 1%r.
     progress.
     apply dtext_ll.
     by rewrite grexpA.
-      by rewrite !grexpA expC.    
+      by rewrite !grexpA expC.   
     rewrite get_set_sameE.
     by rewrite oget_some.
     auto.
@@ -287,23 +285,25 @@ auto.
     proc guess(c : cipher) : bool {RO.f}
   }.
 
-  
-  module INDCPA (Adv : ADV) = {
+
+  module INDCPA (Enc : ENC, Adv : ADV) = {
     module A = Adv(RO)
-    module Enc = HEG(RO)
+    module E = Enc(RO)
 
     proc main() : bool = {
       var x1, x2 : text; var c : cipher; var choice, guess : bool;
       var pubk : group; var privk : exp;
 
+      RO.init();
+
       (* get pubk, similar to initializing EO *)
-      (pubk, privk) <@ Enc.key_gen();
-      
+      (pubk, privk) <@ E.key_gen();
+
 
       (x1,x2) <@ A.choose(pubk);
 
       choice <$ {0,1};
-        c <@ Enc.enc(pubk, choice ? x1 : x2);
+        c <@ E.enc(pubk, choice ? x1 : x2);
 
         guess <@ A.guess(c);
 
@@ -311,7 +311,7 @@ auto.
     }
   }.
 
-  
+
   module type LCDH_ADV = {
     proc main(x1 x2: group) : group fset
   }.
@@ -326,17 +326,74 @@ auto.
       }
     }.
 
-module RO_track : RO = {
+(* based on G2 - see below *)
+
+module Adv2LCDHAdv(Adv : ADV) = {
+  module RO_track : RO = {
+    var mp : (group, text) fmap (* finite map, table *)
+
+    proc init() : unit = {
+    }
+
+    proc f(x : group) : text = {
+        var y : text;
+      if (x \notin mp) { (* not in mp's domain *)
+        y <$ dtext;   (* updating mp so as before but value of *)
+        mp.[x] <- y;  (* x is what we randomly picked *)
+      }
+      return oget mp.[x]; (* mp.[x] is either None or Some t *)
+    }
+  }
+
+  module A = Adv(RO_track)
+
+  proc main(grp1, grp2 : group) : group fset = {
+    var x1, x2 : text; var c : cipher; var choice, guess : bool;
+    var t, y : text;
+
+    RO_track.mp <- empty;
+
+    (x1,x2) <@ A.choose(grp1);
+
+    choice <$ {0,1};
+
+    t <- choice ? x1 : x2;
+
+    y <$ dtext;
+    c <- (grp2, t +^ y);
+
+    guess <@ A.guess(c);
+
+    return fdom RO_track.mp;
+  }
+}.
+
+section.
+
+declare module Adv : ADV{RO, Adv2LCDHAdv}.
+
+axiom Adv_choose_ll :
+  forall (RO <: RO{Adv}),
+  islossless RO.f => islossless Adv(RO).choose.
+
+axiom Adv_guess_ll :
+  forall (RO <: RO{Adv}),
+  islossless RO.f => islossless Adv(RO).guess.
+
+local module RO_track : RO = {
   var mp : (group, text) fmap (* finite map, table *)
   var badHappened : bool
+  var bad_grp : group
 
   proc init() : unit = {
+(*
     mp <- empty;  (* empty map *)
+*)
   }
 
   proc f(x : group) : text = {
       var y : text;
-      if(x \in mp){
+      if (x = bad_grp) {
         badHappened <- true;
       }
     if (x \notin mp) { (* not in mp's domain *)
@@ -346,46 +403,43 @@ module RO_track : RO = {
     return oget mp.[x]; (* mp.[x] is either None or Some t *)
   }
 }.
-  
- module G1 (Adv : ADV) = {
+
+local module G1 = {
     module A = Adv(RO_track)
-    module Enc = HEG(RO_track)
 
     proc main() : bool = {
       var x1, x2 : text; var c : cipher; var choice, guess : bool;
-      var pubk, x : group; var privk : exp;
-       var r : exp;
+      var q1, q2 : exp;
         var u,y,t : text;
 
       (* key_gen but inlined *)
-       privk <$ dexp;
-      pubk <- g ^ privk;
-      
+       q1 <$ dexp;
+       q2 <$ dexp;
 
-      (x1,x2) <@ A.choose(pubk);
+      RO_track.mp <- empty;
+      RO_track.badHappened <- false;
+      RO_track.bad_grp <- g ^ (q1 * q2);
+
+      (x1,x2) <@ A.choose(g ^ q1);
 
         choice <$ {0,1};
 
         (* enc Inlined *)
-       
-        t <- (choice ? x1 : x2);
-        r <$ dexp;
-      (* randomly choosing a u inlined *)
-        u <@ RO.f(pubk ^ r);
 
-        x <- pubk ^ r;
-      
+        t <- (choice ? x1 : x2);
+      (* randomly choosing a u inlined *)
+(*
+        u <@ RO.f(pubk ^ r);
+*)
       (* not sure how to access the same mp while inlining the RO, I think RO.mp works properly *)
-        if (x \notin RO.mp) { (* not in mp's domain *)
+        if (g ^ (q1 * q2) \notin RO_track.mp) { (* not in mp's domain *)
            y <$ dtext;   (* updating mp so as before but value of *)
-           RO.mp.[x] <- y;  (* x is what we randomly picked *)
+           RO_track.mp.[g ^ (q1 * q2)] <- y;  (* x is what we randomly picked *)
         }
 
-      u <- oget RO.mp.[x]; (* mp.[x] is either None or Some t *)
+      u <- oget RO_track.mp.[g ^ (q1 * q2)]; (* mp.[x] is either None or Some t *)
 
-    
-
-    c <- (g ^ r, t +^ u);
+    c <- (g ^ q2, t +^ u);
 
         guess <@ A.guess(c);
 
@@ -393,3 +447,154 @@ module RO_track : RO = {
     }
   }.
 
+local lemma INDCPA_HEG_G1 &m :
+  Pr[INDCPA(HEG, Adv).main() @ &m : res] = Pr[G1.main() @ &m : res].
+proof.
+admit.
+(* use inline, inline*, swap{1} 2 3, swap{2} 2 -1 *)
+qed.
+
+(* to use up to bad reasoning... *)
+
+local module G2 = {
+    module A = Adv(RO_track)
+
+    proc main() : bool = {
+      var x1, x2 : text; var c : cipher; var choice, guess : bool;
+      var q1, q2 : exp;
+        var t, y : text;
+
+      (* key_gen but inlined *)
+       q1 <$ dexp;
+       q2 <$ dexp;
+
+      RO_track.mp <- empty;
+      RO_track.badHappened <- false;
+      RO_track.bad_grp <- g ^ (q1 * q2);
+
+      (x1,x2) <@ A.choose(g ^ q1);
+
+        choice <$ {0,1};
+
+        (* enc Inlined *)
+
+      (* randomly choosing a u inlined *)
+(*
+        u <@ RO.f(pubk ^ r);
+*)
+      (* not sure how to access the same mp while inlining the RO, I think RO.mp works properly *)
+
+           y <$ dtext;   (* updating mp so as before but value of *)
+(*
+           RO_track.mp.[g ^ (q1 * q2)] <- y;  (* x is what we randomly picked *)
+*)
+
+    c <- (g ^ q2, t +^ y);
+
+        guess <@ A.guess(c);
+
+      return choice = guess;
+    }
+  }.
+
+(* up to bad reasoning *)
+
+local lemma G1_G2_eq :
+  equiv[G1.main ~ G2.main :
+        true ==>
+        ={RO_track.badHappened} /\
+        (! RO_track.badHappened{1} => ={res})].
+proof.
+admit. (* look at Sym encryption example, where I first use up to bad
+          reasoning *)
+qed.
+
+local lemma G2_bad_ub &m :
+  Pr[G2.main() @ &m : RO_track.badHappened] =
+  Pr[LCDH(Adv2LCDHAdv(Adv)).main() @ &m : res].
+proof.
+admit.
+qed.
+
+local lemma G1_G2 &m :
+  `|Pr[G1.main() @ &m : res] - Pr[G2.main() @ &m : res]| <=
+  Pr[LCDH(Adv2LCDHAdv(Adv)).main() @ &m : res].
+proof.
+admit. (* look Sym encryption example, where I first use up to bad
+          reasoning *)
+qed.
+
+local module G3 = {
+    module A = Adv(RO_track)
+
+    proc main() : bool = {
+      var x1, x2 : text; var c : cipher; var choice, guess : bool;
+      var q1, q2 : exp;
+      var t, y (*,t*) : text;
+
+      (* key_gen but inlined *)
+       q1 <$ dexp;
+       q2 <$ dexp;
+
+      RO_track.mp <- empty;
+      RO_track.badHappened <- false;
+      RO_track.bad_grp <- g ^ (q1 * q2);
+
+      (x1,x2) <@ A.choose(g ^ q1);
+
+        choice <$ {0,1};
+
+        (* enc Inlined *)
+
+(*
+        t <- (choice ? x1 : x2);
+*)
+        y <$ dtext;   (* updating mp so as before but value of *)
+
+        c <- (g ^ q2, t +^ y); (* because y is one-time pad *)
+
+        guess <@ A.guess(c);
+
+      return choice = guess;
+    }
+  }.
+
+local lemma G2_G3 &m :
+  Pr[G2.main() @ &m : res] = Pr[G3.main() @ &m : res].
+proof.
+admit.  (* one-time pad, just like in labs *)
+qed.
+
+local lemma G3_true &m :
+  Pr[G3.main() @ &m : res] = 1%r / 2%r.
+proof.
+admit.
+qed.
+
+(* sequence of games:
+
+INDCPA(HEG, Adv) <-> G1 <-> G2 <-> G3 = 1%r/2%r
+*)
+
+lemma INDCPA_Sec &m :
+  `|Pr[INDCPA(HEG, Adv).main() @ &m : res] - 1%r / 2%r| <=
+  Pr[LCDH(Adv2LCDHAdv(Adv)).main() @ &m : res].
+proof.
+admit.
+qed.
+
+end section.
+
+print INDCPA_Sec.
+
+lemma INDCPA_Security (Adv <: ADV{RO, Adv2LCDHAdv}) &m :
+  (forall (RO <: RO{Adv}),
+   islossless RO.f => islossless Adv(RO).choose) =>
+  (forall (RO <: RO{Adv}),
+   islossless RO.f => islossless Adv(RO).guess) =>
+  `|Pr[INDCPA(HEG, Adv).main() @ &m : res] - 1%r / 2%r| <=
+  Pr[LCDH(Adv2LCDHAdv(Adv)).main() @ &m : res].
+proof.
+move => Adv_choose_ll Adv_guess_ll.
+apply (INDCPA_Sec Adv Adv_choose_ll Adv_guess_ll &m).
+qed.
